dafny/lectures/lecture5.dfy
@@ -1,0 +1,21 @@
+/**
+sequences are a readonly arrays in dafny, not efficient but proving w/ sequences is easy
+ */
+method {:verify false} Search(q: seq<int>, key: int) returns (i: nat)
+    requires key in q //syntactic suger for (exists i :: 0<= i < |q| && q[i] == key)
+    ensures i < |q| && q[i] == key
+    {
+        i := 0; 
+        while q[i] != key
+            invariant i < |q| && key in q[i..] //q[i...] == the suffix of the array from i
+            decreases |q| - i
+        {
+            assert i < |q| && key in q[i..];
+            assert q[i] != key;
+            // ==> ? NOT before adding the "key in q[i.." to the invariant: (counter example : q=[1],i=0,key = 2, q = [2,3], i = 1, key = 2). 
+            // Although it can't happen, the invariant doesn't know the logic before. So we need to amplify the invriant.
+            assert i+1 < |q| && key in q[i+1..];
+             i:= i+1;
+             assert i < |q| && key in q[i..];
+        }
+    }
