dafny/lectures/lecture8.dfy
@@ -1,0 +1,93 @@
+/**
+ensures forall i :: 0 <= i < a.Length ==> a[i] <= a[i+1] this is not good on its own because we could have changed array's values 
+and not remain with the previous ones. for example array[i] = 7
+we need to add a precondition so that we'll remain with the same.
+ensures forall x :: x in a[..] ==> x in old (a[..]). this is not good because we need to sum the amount of times it's in old_a and a.
+ensures (set x | x in a[..]) == (set x | x in old(a[..])) - more elegant to the ensures above, but the same problem. we need multiset!
+multiset is both a function and a type
+ */
+
+
+predicate Sorted(q: seq<int>)
+{
+    forall i,j :: 0<= i <= j < |q| ==> q[i] <= q[j]
+}
+method InsertionSort(a: array<int>)
+    requires true // pre
+    ensures forall i :: 0 <= i < a.Length -1  ==> a[i] <= a[i+1] 
+    ensures multiset(a[..]) == multiset(old(a[..])) // old a is the value of a in the paramters of the function.
+    modifies a // we can change a, not as in previous functions when they were not part of the frame (can't change local variables). modifies adds to frame.
+    {
+        //introduce logical constants
+        // ghost var A:= multiset(a[..]);
+        ghost var A :| A == multiset(a[..]); // :| is a such that, give me a value of A, such that A == multiset... the same as the assignment above. this is what the law expect (such that)
+        InsertionSort1(a,A);
+
+    }
+    /**
+    Adding ghost to function parameters is only for proving correctness. the compiled version will not show up in running time
+     */
+method InsertionSort1(a:array<int>, ghost A: multiset<int>)
+    requires A == multiset(a[..]) //pre'
+    ensures Sorted(a[..])
+    ensures multiset(a[..]) == multiset(old(a[..])) // == A. the same post condition as inserstion sort.
+    modifies a
+    {
+        //introduce local variable + strengthen postcondition
+        var i;
+        //the guard will not be satisfied and inv will
+        i:= InsertionSort2(a,A);
+        L2(a,i,A);
+    }
+method InsertionSort2(a:array<int>, ghost A: multiset<int>) returns (i: nat)
+    requires A == multiset(a[..])
+    ensures Inv1(a[..],i,A) && !Guard1(a,i,A) // the L2 lemma says it's okay.
+    modifies a
+    {
+        i:=0;
+        while Guard1(a,i,A)
+            invariant Inv1(a[..],i,A)
+            decreases a.Length - i
+            {
+                Insert(a,i,A);
+                i:=i+1;
+
+            }
+    }
+
+method {:verify false} Insert(a:array<int>, i:nat, ghost A: multiset<int>)
+    requires Inv1(a[..],i,A) && Guard1(a,i,A)
+    ensures Inv1(a[..], i+1,A) // for the incrementing of i.
+    modifies a
+/**
+We have began with i <= |q| && Sorted(q[..i]) in Inv1, but there was a problem for Dfny to prove ensures multiset(a[..]) == A in L2
+So we're adding it.
+ */
+predicate Inv1(q: seq<int>, i:nat, A: multiset<int>)
+{
+
+    i <= |q| && Sorted(q[..i]) && multiset(q) == A
+}
+predicate method Guard1(a:array<int>, i:nat, ghost A: multiset<int>)
+{
+    i < a.Length
+}
+/**
+All lemmas's parameters are ghost!
+we need to think about the main loop in the strength post condition.
+ */
+lemma L2(a:array<int>, i:nat, A: multiset<int>)
+    requires Inv1(a[..],i,A) && !Guard1(a,i,A)
+    ensures Sorted(a[..])
+    ensures multiset(a[..]) == A
+
+
+method Main() {
+    var a: array<int> := new int[4];
+    a[0],a[1],a[2],a[3] := 3,8,5,-1;
+    print a[..];
+    ghost var q := a[..]; //ghost variables allows in specification contexts (in asserts and such). they are not real variables (not taking place in memory)
+    InsertionSort(a);
+    assert Sorted(a[..]);
+    assert multiset(a[..]) == multiset(q); // this is why we needed the ghost - instead of old(a) which is undefined in current context. 
+}
